Start substitution lemma for type safety logrel; split into multiple files

stlc/src/lang.lean
@@ -59,51 +59,11 @@ inductive is_many_step : exp → exp → Prop
 | many_steps_transitive (e1 e2 e3:exp) (Hsteps:is_many_step e2 e3) (Hstep:is_step e1 e2)
    : is_many_step e1 e3
 
-def evals_to (e v:exp) : Prop := is_many_step e v ∧ is_val v
-def normalizes (e:exp) : Prop := ∃ v, evals_to e v
-
--- Proof of strong normalization using a logical predicate
-def SN : typ → exp → Prop
-| unitT e := (empty_ctx ⊢ e : unitT) ∧ (normalizes e)
-| (arrowT τ1 τ2) e := (empty_ctx ⊢ e : arrowT τ1 τ2) ∧
-                      (normalizes e) ∧
-                      (∀ (e':exp), (SN τ1 e') → (SN τ2 (ap e e')))
-
 -- Plan is to prove:
 -- a) (∅ ⊢ e:τ) implies SN τ e;
 -- b) SN τ e → normalizes e.
 -- Proving b is easy by induction, it's basically baked into the definition
 -- Proving a by induction on (∅ ⊢ e:τ) will be tricky in the has_type.lam case.
-
-/-
-lemma bad_SN_a :
-  ∀ e τ,
-  empty_ctx ⊢ e:τ →
-  SN τ e :=
-begin
-  introv Hty,
-  generalize h:empty_ctx = Γ,
-  rw h at *,
-  induction Hty; subst h,
-  { -- case: unit
-    sorry,
-  },
-  { -- case: var
-    exfalso, sorry
-  },
-  { -- case: lam abstraction
-    unfold SN,
-    split,
-    { constructor; assumption },
-    split,
-    { sorry },
-    intros a Hsna,
-    rename [Hty_x → x, Hty_e → e, Hty_τ1 → τ1, Hty_τ2 → τ2, Hty_Habs → Habs],
-    sorry,
-  },
-  sorry,
-end
--/
 
 -- def env := finmap (λ _:string, exp)
 def env := list (string × exp)
@@ -113,31 +73,16 @@ def env_sub : env → exp → exp
 | [] e := e
 | (⟨x, ex⟩::l) e := env_sub l (substitute x ex e)
 
--- def env_sub : env → exp → exp
--- | (alist.mk [] _) e := e
--- | (alist.mk (⟨x, ex⟩ :: l) nd) e := env_sub (alist.mk l (list.nodupkeys_cons.1 nd).2) (substitute x ex e)
-
 instance env_has_mem : has_mem (string × exp) env := list.has_mem
-
--- noncomputable def env_sub : env → exp → exp
--- | γ e :=
---   match (γ.entries.to_list) with
---   | [] := e
---   | ((sigma.mk x ex) :: l) := (substitute x ex e)
---   end
-
--- def is_env_ctx : env → context → Prop
--- | γ Γ := ∀ x v, (x,v) ∈ γ → (∃ τ, Γ x = some τ ∧ SN τ v)
--- | γ Γ := ∀ x τ,  Γ x = some τ → (∃ v, (x,v) ∈ γ ∧ SN τ v)
 
 def context_list := list (string × typ)
 def mk_context : context_list → context
 | [] := empty_ctx
 | ((x,τ) :: ctx) := (x↦τ; mk_context ctx)
 
-def is_env_ctx : env → context_list → Prop
+def is_env_ctx (P:typ → exp → Prop) : env → context_list → Prop
 | [] [] := true
-| ((x,v)::γ) ((y,τ)::Γ) := x=y ∧ is_env_ctx γ Γ ∧ SN τ v
+| ((x,v)::γ) ((y,τ)::Γ) := x=y ∧ is_env_ctx γ Γ ∧ P τ v
 | _ _ := false
 
 -- FIXME: copy/paste from e-lang
@@ -263,14 +208,15 @@ begin
 end
 
 lemma substitution_property :
-  ∀ γ Γ c e τ ,
-  is_env_ctx γ c →
+  ∀ γ Γ c e τ P,
+  is_env_ctx P γ c →
+  (∀ v' τ', (P τ' v') → (empty_ctx ⊢ v' : τ')) →
   Γ = mk_context c →
   Γ ⊢ e : τ →
   empty_ctx ⊢ env_sub γ e : τ
   :=
 begin
-  introv Henv HΓ Hty,
+  introv Henv Hclosed HΓ Hty,
   subst HΓ,
   induction γ generalizing c e,
   {
@@ -291,86 +237,7 @@ begin
   apply sub_property,
   tactic.swap,
   { exact Hty, },
-  { cases c_hd_snd; cases Henv with _ Hsn; apply Hsn.1 },
-end
-
-lemma sn_implies_normalizes :
-∀ e τ, SN τ e → normalizes e :=
-begin
- introv Hsn,
- cases τ, exact Hsn.2, exact Hsn.2.1
-end
-
-lemma sn_preservation :
-  ∀ e e' τ,
-  empty_ctx ⊢ e : τ →
-  (e ↦str e') →
-  (SN τ e' → SN τ e) -- ∧ (SN τ e → SN τ e')
-:=
-begin
-introv Hty Hstep,
-{ -- backwards preservation
-  intros Hsn,
-  generalize h : (empty_ctx = Γ),
-  rw h at *,
-  -- induction Hty generalizing e'; subst h,
-  induction τ generalizing e' e; subst h,
-  -- cases Hstep,
-  -- induction Hty; subst h,
-  {
-    unfold SN,
-    split, assumption,
-    have h := (sn_implies_normalizes _ _ Hsn),
-    cases h,
-    existsi h_w,
-    unfold evals_to at *,
-    split,
-    { apply is_many_step.many_steps_transitive,
-      apply h_h.1, assumption
-    },
-    apply h_h.2,
-  },
-  { unfold SN,
-    split,
-    { assumption },
-    split,
-    {
-      have h := (sn_implies_normalizes _ _ Hsn),
-      cases h,
-      existsi h_w,
-      unfold evals_to at *,
-      cases h_h,
-      split,
-      {
-        apply is_many_step.many_steps_transitive,
-        { assumption },
-        assumption
-      },
-      assumption
-    },
-    cases Hstep,
-    {
-      unfold SN at Hsn,
-      intros a Hsna,
-      apply τ_ih_τ2,
-      { constructor, assumption  },
-      { apply Hsn.2.2, assumption },
-      constructor,
-      { assumption },
-      cases τ_τ1; apply Hsna.1,
-    },
-    {
-      intros a Hsna,
-      unfold SN at Hsn,
-      apply τ_ih_τ2,
-      { constructor, assumption },
-      { apply Hsn.2.2, assumption },
-      constructor,
-      { assumption },
-      cases τ_τ1; apply Hsna.1,
-    }
-  },
-},
+  { cases c_hd_snd; cases Henv with _ Hsn; apply Hclosed; apply Hsn },
 end
 
 lemma env_sub_unit :
@@ -442,49 +309,44 @@ begin
   },
 end
 
-lemma env_sub_sn :
-∀ γ v τ, SN τ v → env_sub γ v = v :=
+lemma env_sub_closed :
+∀ γ v τ, (empty_ctx ⊢ v : τ) → env_sub γ v = v :=
 begin
   introv Hsn,
-  have h : (empty_ctx ⊢ v : τ),
-  {
-    cases τ; exact Hsn.1
-  },
-  clear Hsn,
   generalize h : empty_ctx = Γ,
   rw h at *,
-  induction h generalizing γ; subst h,
+  induction Hsn generalizing γ; subst h,
   { apply env_sub_unit },
-  { exfalso, unfold empty_ctx at h_Hvar, contradiction },
+  { exfalso, unfold empty_ctx at Hsn_Hvar, contradiction },
   {
     induction γ,
     { unfold env_sub },
     cases γ_hd,
     unfold env_sub,
     unfold substitute,
-    by_cases (γ_hd_fst = h_x),
+    by_cases (γ_hd_fst = Hsn_x),
     { simp * },
     { rw if_neg, tactic.swap, trivial,
       rw sub_lam_ne,
       { apply γ_ih },
       tactic.swap, assumption,
-      { intros, unfold update_context at *, by_cases h_x = x,
+      { intros, unfold update_context at *, by_cases Hsn_x = x,
         { simp *, subst h, tauto },
         { rw if_neg at *, unfold empty_ctx at *, contradiction, assumption }
       }
     }
   },
   { rw env_sub_ap,
-    rw h_ih_Hfunc,
-    rw h_ih_Hargs,
+    rw Hsn_ih_Hfunc,
+    rw Hsn_ih_Hargs,
     repeat { trivial },
   },
 end
 
 lemma double_substitute :
 ∀ x τ1 τ2 ex1 ex2 e,
-SN τ1 ex1 →
-SN τ2 ex2 →
+empty_ctx ⊢ ex1 : τ1 →
+empty_ctx ⊢ ex2 : τ2 →
 (substitute x ex2 (substitute x ex1 e)) = substitute x ex1 e :=
 begin
 intros,
@@ -494,7 +356,7 @@ intros,
       have h : (substitute e ex2 ex1 = env_sub [(e,ex2)] ex1),
       { unfold env_sub },
       rw h,
-      rw env_sub_sn,
+      rw env_sub_closed,
       assumption
     },
     {
@@ -520,8 +382,8 @@ end
 
 lemma substitute_commute :
 ∀ x y τx τy ex ey e,
-SN τx ex →
-SN τy ey →
+(empty_ctx ⊢ ex : τx) →
+(empty_ctx ⊢ ey : τy) →
 x ≠ y →
 (substitute x ex (substitute y ey e)) = (substitute y ey (substitute x ex e)) :=
 begin
@@ -536,7 +398,7 @@ begin
       simp *,
       have h : (substitute x ex ey = env_sub [(x,ex)] ey),
       { unfold env_sub },
-      rw h, apply env_sub_sn, assumption
+      rw h, apply env_sub_closed, assumption
     },
     {
       rw if_neg, tactic.swap, trivial,
@@ -546,7 +408,7 @@ begin
         simp *,
         have h : (substitute y ey ex = env_sub [(y,ey)] ex),
         { unfold env_sub },
-        rw h, rw env_sub_sn, assumption
+        rw h, rw env_sub_closed, assumption
       },
       {
         rw if_neg, unfold substitute, rw if_neg, repeat { assumption }
@@ -571,172 +433,3 @@ begin
   }
 end
 
--- XXX: this is a tricky lemma because of variable shadowing. If we worked
--- modulo α-equivalence, this trickiness might be avoided.
-lemma env_sub_lam_step :
-∀ γ c x τ1 e e',
-is_env_ctx γ c →
-SN τ1 e' →
-(env_sub γ (lam x τ1 e)).ap e' ↦str (env_sub γ (substitute x e' e)) :=
-begin
-  introv Hctx Hsn,
-  induction γ generalizing e c,
-  { unfold env_sub, constructor },
-  cases γ_hd with y vy,
-  unfold env_sub,
-  unfold substitute,
-  by_cases (y = x),
-  {
-    simp *,
-    cases c,
-    { exfalso, unfold is_env_ctx at *, assumption },
-    cases c_hd,
-    unfold is_env_ctx at Hctx,
-    rw double_substitute,
-    { apply γ_ih, apply Hctx.2.1 },
-    { assumption },
-    { apply Hctx.2.2 },
-  },
-  {
-    rw if_neg, tactic.swap, tauto,
-    cases c,
-    { exfalso, unfold is_env_ctx at *, assumption },
-    cases c_hd,
-    unfold is_env_ctx at Hctx,
-    rw substitute_commute,
-    {
-      apply γ_ih,
-      { apply Hctx.2.1 },
-    },
-    { apply Hctx.2.2 },
-    { assumption },
-    { assumption },
-  }
-end
-
-theorem sn_general :
-  ∀ Γ c γ e τ,
-  Γ = mk_context c →
-  Γ ⊢ e : τ →
-  is_env_ctx γ c →
-  SN τ (env_sub γ e) :=
-begin
-  introv HΓ Hty Henv,
-  induction Hty generalizing γ c; subst HΓ,
-  { -- case: unit
-    rw env_sub_unit,
-    unfold SN,
-    split,
-    { constructor },
-    existsi exp.unit,
-    unfold evals_to,
-    split; constructor
-  },
-  { -- case: var
-    induction γ generalizing c,
-    {
-      induction c,
-      { exfalso, contradiction },
-      { exfalso, unfold is_env_ctx at *, contradiction }
-    },
-    induction c,
-    { exfalso, contradiction },
-    cases γ_hd, cases c_hd,
-    unfold is_env_ctx at *,
-    unfold env_sub,
-    cases Henv with Hre Henv,
-    subst Hre,
-    by_cases (Hty_x = γ_hd_fst),
-    { -- the first thing in Γ/γ is the var Hty_x
-      subst h,
-      unfold env_sub substitute at c_ih,
-      unfold substitute at *,
-      simp * at *,
-      unfold mk_context update_context at Hty_Hvar,
-      simp * at Hty_Hvar,
-      injection Hty_Hvar,
-      subst h_1,
-      rw (env_sub_sn _ _ _ Henv.2),
-      apply Henv.2
-    },
-    { -- induction
-      unfold substitute, rw if_neg,
-      tactic.swap, { tauto, },
-      unfold mk_context update_context at Hty_Hvar,
-      rw if_neg at Hty_Hvar,
-      tactic.swap, { tauto },
-      apply γ_ih,
-      { apply Henv.1, },
-      { assumption }
-    },
-  },
-  { -- case: lam. This is the tricky case
-    rename [Hty_x → x, Hty_τ1→τ1, Hty_τ2→τ2, Hty_e→e],
-    unfold SN,
-    split,
-    { -- property 1 in notes
-      apply substitution_property,
-      { assumption },
-      { refl },
-      constructor, assumption
-    },
-    split,
-    { -- property 2 in notes
-      existsi _,
-      unfold evals_to,
-      split,
-      apply is_many_step.many_steps_reflexive,
-      apply env_sub_lam_val,
-    },
-    -- property 3
-    intros e' Hsn,
-    have h := (sn_implies_normalizes _ _ Hsn),
-    cases h with w Heval,
-    cases Heval with Hsteps Hval,
-
-    apply (sn_preservation _ _ τ2 _ _),
-    tactic.rotate 2,
-    {
-      constructor,
-      { apply substitution_property,
-        assumption, refl, constructor, assumption
-      },
-      cases τ1; apply Hsn.1, -- this could be a separate lemma
-    },
-    {
-      apply env_sub_lam_step,
-      { assumption },
-      { assumption }
-    },
-    -- XXX: here, our proof diverges from the notes because we are doing
-    -- call-by-name but the notes are doing call-by-value
-
-    have h: (env_sub ((x,e')::γ) e) = (env_sub γ (substitute x e' e)),
-    { unfold env_sub },
-    rw <- h,
-    apply Hty_ih _ ((x, τ1) :: c),
-    { unfold mk_context },
-    unfold is_env_ctx,
-    split, refl,
-    split, assumption,
-    assumption,
-  },
-  { -- case: ap
-    specialize Hty_ih_Hfunc _ _ _ Henv, trivial,
-    specialize Hty_ih_Hargs _ _ _ Henv, trivial,
-    unfold SN at Hty_ih_Hfunc,
-    rw env_sub_ap,
-    apply Hty_ih_Hfunc.2.2,
-    apply Hty_ih_Hargs
-  }
-end
-
-theorem strong_normalization :
-  ∀ e τ, (empty_ctx ⊢ e : τ) → normalizes e :=
-begin
-  introv Hty,
-  have h := (sn_general empty_ctx [] [] e τ _ Hty _),
-  { apply sn_implies_normalizes, assumption },
-  { unfold mk_context },
-  { unfold is_env_ctx },
-end
