stlc/src/normalization.lean
@@ -1,0 +1,273 @@
+import lang
+
+open typ exp
+
+def evals_to (e v:exp) : Prop := is_many_step e v ∧ is_val v
+def normalizes (e:exp) : Prop := ∃ v, evals_to e v
+
+-- Proof of strong normalization using a logical predicate
+def SN : typ → exp → Prop
+| unitT e := (empty_ctx ⊢ e : unitT) ∧ (normalizes e)
+| (arrowT τ1 τ2) e := (empty_ctx ⊢ e : arrowT τ1 τ2) ∧
+                      (normalizes e) ∧
+                      (∀ (e':exp), (SN τ1 e') → (SN τ2 (ap e e')))
+
+lemma sn_implies_closed :
+∀ e τ,
+ SN τ e → empty_ctx ⊢ e : τ :=
+begin
+  intros,
+  cases τ; unfold SN at *; tauto
+end
+
+lemma sn_implies_normalizes :
+∀ e τ, SN τ e → normalizes e :=
+begin
+ introv Hsn,
+ cases τ, exact Hsn.2, exact Hsn.2.1
+end
+
+lemma sn_preservation :
+  ∀ e e' τ,
+  empty_ctx ⊢ e : τ →
+  (e ↦str e') →
+  (SN τ e' → SN τ e) -- ∧ (SN τ e → SN τ e')
+:=
+begin
+introv Hty Hstep,
+{ -- backwards preservation
+  intros Hsn,
+  generalize h : (empty_ctx = Γ),
+  rw h at *,
+  -- induction Hty generalizing e'; subst h,
+  induction τ generalizing e' e; subst h,
+  -- cases Hstep,
+  -- induction Hty; subst h,
+  {
+    unfold SN,
+    split, assumption,
+    have h := (sn_implies_normalizes _ _ Hsn),
+    cases h,
+    existsi h_w,
+    unfold evals_to at *,
+    split,
+    { apply is_many_step.many_steps_transitive,
+      apply h_h.1, assumption
+    },
+    apply h_h.2,
+  },
+  { unfold SN,
+    split,
+    { assumption },
+    split,
+    {
+      have h := (sn_implies_normalizes _ _ Hsn),
+      cases h,
+      existsi h_w,
+      unfold evals_to at *,
+      cases h_h,
+      split,
+      {
+        apply is_many_step.many_steps_transitive,
+        { assumption },
+        assumption
+      },
+      assumption
+    },
+    cases Hstep,
+    {
+      unfold SN at Hsn,
+      intros a Hsna,
+      apply τ_ih_τ2,
+      { constructor, assumption  },
+      { apply Hsn.2.2, assumption },
+      constructor,
+      { assumption },
+      cases τ_τ1; apply Hsna.1,
+    },
+    {
+      intros a Hsna,
+      unfold SN at Hsn,
+      apply τ_ih_τ2,
+      { constructor, assumption },
+      { apply Hsn.2.2, assumption },
+      constructor,
+      { assumption },
+      cases τ_τ1; apply Hsna.1,
+    }
+  },
+},
+end
+
+-- XXX: this is a tricky lemma because of variable shadowing. If we worked
+-- modulo α-equivalence, this trickiness might be avoided.
+lemma env_sub_lam_step :
+∀ γ c x τ1 e e',
+is_env_ctx SN γ c →
+SN τ1 e' →
+(env_sub γ (lam x τ1 e)).ap e' ↦str (env_sub γ (substitute x e' e)) :=
+begin
+  introv Hctx Hsn,
+  induction γ generalizing e c,
+  { unfold env_sub, constructor },
+  cases γ_hd with y vy,
+  unfold env_sub,
+  unfold substitute,
+  by_cases (y = x),
+  {
+    simp *,
+    cases c,
+    { exfalso, unfold is_env_ctx at *, assumption },
+    cases c_hd,
+    unfold is_env_ctx at Hctx,
+    rw double_substitute,
+    { apply γ_ih, apply Hctx.2.1 },
+    { apply sn_implies_closed, assumption },
+    { apply sn_implies_closed, apply Hctx.2.2 },
+  },
+  {
+    rw if_neg, tactic.swap, tauto,
+    cases c,
+    { exfalso, unfold is_env_ctx at *, assumption },
+    cases c_hd,
+    unfold is_env_ctx at Hctx,
+    rw substitute_commute,
+    {
+      apply γ_ih,
+      { apply Hctx.2.1 },
+    },
+    { apply sn_implies_closed, apply Hctx.2.2 },
+    { apply sn_implies_closed, assumption },
+    { assumption },
+  }
+end
+
+theorem sn_general :
+  ∀ Γ c γ e τ,
+  Γ = mk_context c →
+  Γ ⊢ e : τ →
+  is_env_ctx SN γ c →
+  SN τ (env_sub γ e) :=
+begin
+  introv HΓ Hty Henv,
+  induction Hty generalizing γ c; subst HΓ,
+  { -- case: unit
+    rw env_sub_unit,
+    unfold SN,
+    split,
+    { constructor },
+    existsi exp.unit,
+    unfold evals_to,
+    split; constructor
+  },
+  { -- case: var
+    induction γ generalizing c,
+    {
+      induction c,
+      { exfalso, contradiction },
+      { exfalso, unfold is_env_ctx at *, contradiction }
+    },
+    induction c,
+    { exfalso, contradiction },
+    cases γ_hd, cases c_hd,
+    unfold is_env_ctx at *,
+    unfold env_sub,
+    cases Henv with Hre Henv,
+    subst Hre,
+    by_cases (Hty_x = γ_hd_fst),
+    { -- the first thing in Γ/γ is the var Hty_x
+      subst h,
+      unfold env_sub substitute at c_ih,
+      unfold substitute at *,
+      simp * at *,
+      unfold mk_context update_context at Hty_Hvar,
+      simp * at Hty_Hvar,
+      injection Hty_Hvar,
+      subst h_1,
+      rw (env_sub_closed _ _ _ _),
+      { apply Henv.2 },
+      tactic.swap, { apply sn_implies_closed, apply Henv.2 },
+    },
+    { -- induction
+      unfold substitute, rw if_neg,
+      tactic.swap, { tauto, },
+      unfold mk_context update_context at Hty_Hvar,
+      rw if_neg at Hty_Hvar,
+      tactic.swap, { tauto },
+      apply γ_ih,
+      { apply Henv.1, },
+      { assumption }
+    },
+  },
+  { -- case: lam. This is the tricky case
+    rename [Hty_x → x, Hty_τ1→τ1, Hty_τ2→τ2, Hty_e→e],
+    unfold SN,
+    split,
+    { -- property 1 in notes
+      apply substitution_property,
+      { assumption },
+      { intros, apply sn_implies_closed, assumption },
+      { refl },
+      constructor, assumption
+    },
+    split,
+    { -- property 2 in notes
+      existsi _,
+      unfold evals_to,
+      split,
+      apply is_many_step.many_steps_reflexive,
+      apply env_sub_lam_val,
+    },
+    -- property 3
+    intros e' Hsn,
+    have h := (sn_implies_normalizes _ _ Hsn),
+    cases h with w Heval,
+    cases Heval with Hsteps Hval,
+
+    apply (sn_preservation _ _ τ2 _ _),
+    tactic.rotate 2,
+    {
+      constructor,
+      { apply substitution_property,
+        assumption, apply sn_implies_closed,
+        refl, constructor, assumption
+      },
+      cases τ1; apply Hsn.1, -- this could be a separate lemma
+    },
+    {
+      apply env_sub_lam_step,
+      { assumption },
+      { assumption }
+    },
+    -- XXX: here, our proof diverges from the notes because we are doing
+    -- call-by-name but the notes are doing call-by-value
+
+    have h: (env_sub ((x,e')::γ) e) = (env_sub γ (substitute x e' e)),
+    { unfold env_sub },
+    rw <- h,
+    apply Hty_ih _ ((x, τ1) :: c),
+    { unfold mk_context },
+    unfold is_env_ctx,
+    split, refl,
+    split, assumption,
+    assumption,
+  },
+  { -- case: ap
+    specialize Hty_ih_Hfunc _ _ _ Henv, trivial,
+    specialize Hty_ih_Hargs _ _ _ Henv, trivial,
+    unfold SN at Hty_ih_Hfunc,
+    rw env_sub_ap,
+    apply Hty_ih_Hfunc.2.2,
+    apply Hty_ih_Hargs
+  }
+end
+
+theorem strong_normalization :
+  ∀ e τ, (empty_ctx ⊢ e : τ) → normalizes e :=
+begin
+  introv Hty,
+  have h := (sn_general empty_ctx [] [] e τ _ Hty _),
+  { apply sn_implies_normalizes, assumption },
+  { unfold mk_context },
+  { unfold is_env_ctx },
+end
